src/examplelang/lang.v
@@ -1,0 +1,132 @@
+From ITree Require Import ITree.
+From stdpp Require Import strings binders.
+
+From iris.itree Require Import wpi choice angelic_choice ub heap handler itree.
+From iris.itree.threadpool Require Import handler.
+
+Inductive base_lit : Set :=
+  | LitInt (n : Z)
+  | LitLoc (l : loc).
+
+Inductive expr :=
+  | Val (v : val)
+  | Var (x : string)
+  | Lam (x : binder) (e : expr)
+  | App (e1 e2 : expr)
+  | Plus (e1 e2 : expr)
+  | If (e0 e1 e2 : expr)
+  | Ref (e : expr)
+  | Load (e : expr)
+  | Store (e1 e2 : expr)
+  | PickInt
+  | Spawn (e : expr)
+with val :=
+  | LitV (l : base_lit)
+  | LamV (x : binder) (e : expr).
+
+(** Substitution *)
+Fixpoint subst (x : string) (v : val) (e : expr) : expr :=
+  match e with
+  | Val _ => e
+  | Var y => if decide (x = y) then Val v else Var y
+  | Lam y e =>
+     Lam y $ if decide (BNamed x ≠ y) then subst x v e else e
+  | App e1 e2 => App (subst x v e1) (subst x v e2)
+  | Plus e1 e2 => Plus (subst x v e1) (subst x v e2)
+  | If e0 e1 e2 => If (subst x v e0) (subst x v e1) (subst x v e2)
+  | Ref e => Ref (subst x v e)
+  | Load e => Load (subst x v e)
+  | Store e1 e2 => Store (subst x v e1) (subst x v e2)
+  | PickInt => PickInt
+  | Spawn e => Spawn (subst x v e)
+  end.
+
+Definition subst' (mx : binder) (v : val) : expr → expr :=
+  match mx with BNamed x => subst x v | BAnon => id end.
+
+Definition exampleE : Type → Type := threadpoolE +' ubE +' heapE val +' demonicE +' angelicE.
+Global Hint Transparent exampleE : itree_auto.
+
+(** Cast a value to [LamV]. *)
+Definition val_to_LamV (v : val) : option (binder * expr) :=
+  match v with
+  | LamV x_ e => Some (x_, e)
+  | _ => None
+  end.
+(** Cast a value to [LitInt]. *)
+Definition val_to_int (v : val) : option Z :=
+  match v with
+  | LitV (LitInt n) => Some n
+  | _ => None
+  end.
+(** Cast a value to [LitLoc]. *)
+Definition val_to_loc (v : val) : option loc :=
+  match v with
+  | LitV (LitLoc l) => Some l
+  | _ => None
+  end.
+
+Definition yield_if_not_val (e : expr) {E} `{threadpoolE -< E} : itree E () :=
+  match e with
+  | Val _ => Ret ()
+  | _ => yield
+  end.
+Arguments yield_if_not_val !_ / _.
+
+Lemma yield_if_not_val_to_translate {E1 E2} (e : expr) (HE1 : threadpoolE -< E1) (HE2 : threadpoolE -< E2) (Hin : E1 -< E2) :
+  TranslateReSum Hin HE1 HE2 →
+  ITreeToTranslate (yield_if_not_val e) Hin (yield_if_not_val e).
+Proof. move => ?. by destruct e => /=; try apply Ret_to_translate; apply yield_to_translate. Qed.
+Global Hint Resolve yield_if_not_val_to_translate : itree_auto.
+
+Fixpoint compile_expr' (e : expr) : itree (callE expr val +' exampleE) val :=
+  let compile_expr_yield e := (v ← compile_expr' e ; yield_if_not_val e ;; Ret v)%itree in
+  match e with
+  | Var _ => ub
+  | Val v => Ret v
+  | Lam x e => Ret (LamV x e)
+  | App e1 e2 =>
+      f ← compile_expr_yield e1;
+      v ← compile_expr_yield e2;
+      '(x_, e) ← (val_to_LamV f)?;
+      let body := subst' x_ v e in
+      yield_if_not_val body;;
+      call body
+  | Plus e1 e2 =>
+      v1 ← compile_expr_yield e1;
+      v2 ← compile_expr_yield e2;
+      n1 ← (val_to_int v1)?;
+      n2 ← (val_to_int v2)?;
+      Ret (LitV (LitInt (n1 + n2)))
+  | If e0 e1 e2 =>
+      v ← compile_expr_yield e0;
+      n ← (val_to_int v)?;
+      if decide (n ≠ 0) then
+        yield_if_not_val e1;;
+        compile_expr' e1
+      else
+        yield_if_not_val e2;;
+        compile_expr' e2
+  | Ref e =>
+      v ← compile_expr_yield e;
+      l ← alloc v;
+      Ret (LitV (LitLoc l))
+  | Load e =>
+      l' ← compile_expr_yield e;
+      l ← (val_to_loc l')?;
+      v ← load_or_ub l;
+      Ret v
+  | Store e1 e2 =>
+      l' ← compile_expr_yield e1;
+      v ← compile_expr_yield e2;
+      l ← (val_to_loc l')?;
+      store_or_ub l v
+  | PickInt =>
+      n ← angelic_choice Z;
+      Ret (LitV (LitInt n))
+  | Spawn e =>
+      spawn (compile_expr_yield e ;; Ret ()) ;;
+      Ret (LitV (LitInt 0))
+  end%itree.
+
+Definition compile_expr : expr → itree exampleE val := rec compile_expr'.
