src/examplelang/program_logic.v
@@ -1,0 +1,187 @@
+From ITree Require Import ITree Recursion RecursionFacts InterpFacts Eqit.
+From elpi.apps Require Import locker.
+From iris Require Import prelude.
+From iris.proofmode Require Import proofmode.
+From iris.base_logic Require Import ghost_map invariants.
+From iris.bi Require Import weakestpre.
+
+From iris.itree Require Import wpi choice angelic_choice ub heap handler itree.
+From iris.itree.threadpool Require Import handler.
+From iris.itree.examplelang Require Import lang.
+
+Class exampleHGpreS (Σ : gFunctors) := ExampleHGpreS {
+  exampleH_heapHG :> heapHGpreS Σ val;
+}.
+Local Existing Instances exampleH_heapHG.
+Class exampleHGS (Σ : gFunctors) := ExampleHGS {
+  exampleH_heapHGS :> heapHGS Σ val;
+}.
+Local Existing Instances exampleH_heapHGS.
+
+Section handler.
+  Context {Σ} `{!invGS_gen hlc Σ} `{!exampleHGS Σ}.
+
+  Definition exampleH : iHandler Σ exampleE :=
+    threadpoolH ⊕ ubH ⊕ heapH val ⊕ demonicH ⊕ angelicH.
+
+  Lemma wpi_yield_if_not_val e Φ :
+    Φ tt -∗
+    WPi yield_if_not_val e @ exampleH; ⊤ {{ Φ }}.
+  Proof.
+    iIntros "HΦ". rewrite /yield_if_not_val.
+    case_match; try by iApply @wpi_yield.
+    by iApply wpi_ret.
+  Qed.
+End handler.
+
+(** Weakest precondition abstraction for heaplang expressions. *)
+lock Definition wp_example `{!invGS_gen hlc Σ} `{!exampleHGS Σ} :
+  Wp (iProp Σ) expr val stuckness := λ _ E e Φ,
+    (WPi compile_expr e @ exampleH; E {{ Φ }})%I.
+Global Existing Instance wp_example.
+
+Section wp.
+  Context `{!invGS_gen hlc Σ} `{!exampleHGS Σ}.
+
+  Lemma wp_unfold e E Φ :
+    WP e @ E {{ Φ }} ⊣⊢
+    WPi compile_expr e @ exampleH; E {{ Φ }}.
+  Proof. by rewrite unlock. Qed.
+
+  Lemma wp_wand E e Φ Ψ :
+    (∀ v, Φ v -∗ Ψ v) -∗
+    WP e @ E {{ Φ }} -∗ WP e @ E {{ Ψ }}.
+  Proof.
+    iIntros "Hwp". rewrite !wp_unfold.
+    by iApply wpi_wand.
+  Qed.
+
+  Lemma wp_frame P E e Φ :
+    P -∗
+    WP e @ E {{ Φ }} -∗ WP e @ E {{ v, P ∗ Φ v }}.
+  Proof.
+    iIntros "HP Hwp". iApply (wp_wand with "[HP]"); last eauto.
+    iIntros (v) "HΦ". iFrame.
+  Qed.
+
+  Lemma wp_val E v Φ :
+    Φ v -∗
+    WP Val v @ E {{ Φ }}.
+  Proof.
+    iIntros "Hwp". rewrite !wp_unfold.
+    rewrite /compile_expr. wpi_norm/=.
+    by iApply wpi_ret.
+  Qed.
+
+  Lemma wp_bind_plus_l e1 e2 Φ :
+    WP e1 @ ⊤ {{ v1, WP (Plus (Val v1) e2) @ ⊤ {{ Φ }} }} -∗
+    WP Plus e1 e2 @ ⊤ {{ Φ }}.
+  Proof.
+    iIntros "Hwp". rewrite !wp_unfold.
+    rewrite /compile_expr. wpi_norm/=.
+    iApply wpi_bind. rewrite rec_as_interp.
+    iApply wpi_wand; last done.
+    iIntros (r) "Hwp". iApply wpi_bind. iApply wpi_yield_if_not_val.
+    rewrite !wp_unfold. rewrite /compile_expr rec_as_interp. by wpi_norm/= in "Hwp".
+  Qed.
+
+  Lemma wp_bind_plus_r v1 e2 Φ :
+    WP e2 @ ⊤ {{ v2, WP (Plus (Val v1) (Val v2)) @ ⊤ {{ Φ }} }} -∗
+    WP Plus (Val v1) e2 @ ⊤ {{ Φ }}.
+  Proof.
+    iIntros "Hwp". rewrite !wp_unfold.
+    rewrite /compile_expr. wpi_norm/=.
+    iApply wpi_bind. rewrite rec_as_interp.
+    iApply wpi_wand; last done.
+    iIntros (r) "Hwp". iApply wpi_bind. iApply wpi_yield_if_not_val.
+    rewrite !wp_unfold. rewrite /compile_expr rec_as_interp. by wpi_norm/= in "Hwp".
+  Qed.
+
+  Lemma wp_plus E n m Φ :
+    Φ (LitV (LitInt (n + m))) -∗
+    WP Plus (Val (LitV (LitInt n))) (Val (LitV (LitInt m))) @ E {{ Φ }}.
+  Proof.
+    iIntros "HΦ". rewrite wp_unfold.
+    rewrite /compile_expr. wpi_norm/=. by iApply wpi_ret.
+  Qed.
+
+  Lemma wp_app x_ v e Φ :
+    WP subst' x_ v  e @ ⊤ {{ Φ }} -∗
+    WP App (Val (LamV x_ e)) (Val v) @ ⊤ {{ Φ }}.
+  Proof.
+    iIntros "Hwp". rewrite !wp_unfold.
+    rewrite /compile_expr. wpi_norm/=.
+    iApply wpi_bind. iApply wpi_yield_if_not_val.
+    rewrite interp_recursive_call //.
+  Qed.
+
+  Lemma wp_if_true e1 e2 (n : Z) Φ :
+    n ≠ 0 →
+    WP e1 @ ⊤ {{ Φ }} -∗
+    WP If (Val (LitV (LitInt n))) e1 e2 @ ⊤ {{ Φ }}.
+  Proof.
+    iIntros (Hneq) "Hwp". rewrite !wp_unfold.
+    rewrite /compile_expr. wpi_norm/=. rewrite decide_True //.
+    wpi_norm/=. iApply wpi_bind. iApply wpi_yield_if_not_val.
+    rewrite rec_as_interp //.
+  Qed.
+
+  Lemma wp_if_false e1 e2 Φ :
+    WP e2 @ ⊤ {{ Φ }} -∗
+    WP If (Val (LitV (LitInt 0))) e1 e2 @ ⊤ {{ Φ }}.
+  Proof.
+    iIntros "Hwp". rewrite !wp_unfold.
+    rewrite /compile_expr. wpi_norm/=.
+    wpi_norm/=. iApply wpi_bind. iApply wpi_yield_if_not_val.
+    rewrite rec_as_interp //.
+  Qed.
+
+  Lemma wp_ref E v Φ :
+    ↑heapH_inv_name ⊆ E →
+    (∀ l,
+       l ↦ v -∗
+       Φ (LitV (LitLoc l)))
+    -∗
+    WP Ref (Val v) @ E {{ Φ }}.
+  Proof.
+    iIntros (Hmask) "Hwand".
+    rewrite wp_unfold /compile_expr. wpi_norm/=.
+    iApply wpi_bind. Set Typeclasses Debug. wpi_norm. iApply @wpi_alloc; first done.
+    iIntros (l) "Hpointsto". iApply wpi_ret.
+    by iApply "Hwand".
+  Qed.
+
+  Lemma wp_load E l v dq Φ :
+    ↑heapH_inv_name ⊆ E →
+    l ↦{dq} v -∗
+    (l ↦{dq} v -∗ Φ v) -∗
+    WP Load (Val $ LitV $ LitLoc l) @ E {{ Φ }}.
+  Proof.
+    iIntros (Hmask) "Hmapsto Hwand".
+    rewrite wp_unfold /compile_expr. wpi_norm/=.
+    by iApply (@wpi_load_or_ub with "Hmapsto").
+  Qed.
+
+  Lemma wp_pick_int E Φ :
+    (∃ n, Φ (LitV (LitInt n))) -∗
+    WP PickInt @ E {{ Φ }}.
+  Proof.
+    iIntros "Hwp". rewrite !wp_unfold.
+    rewrite /compile_expr. wpi_norm/=.
+    iApply wpi_bind. iDestruct "Hwp" as "[%n HΦ]". iApply @wpi_angelic.
+    iApply wpi_ret. by iApply wpi_ret.
+  Qed.
+
+  Lemma wp_spawn E e Φ :
+    Φ (LitV (LitInt 0))  -∗
+    WP e @ ⊤ {{ _, True }} -∗
+    WP Spawn e @ E {{ Φ }}.
+  Proof.
+    iIntros "HΦ Hwp". rewrite !wp_unfold.
+    rewrite /compile_expr. (* TODO: Make this work: Set Typeclasses Debug Verbosity 2. wpi_norm/=. *)
+    wpi_norm/=. iApply wpi_bind. iApply (@wpi_spawn with "[HΦ]").
+    - by iApply wpi_ret.
+    - wpi_norm/=. iApply wpi_bind. rewrite rec_as_interp. iApply wpi_wand; last done.
+      iIntros (r) "_". iApply wpi_bind. iApply wpi_yield_if_not_val. by iApply wpi_ret.
+  Qed.
+End wp.
